proof/theories/Optimize.v
@@ -22,11 +22,18 @@ Import ListNotations.
 
 Definition field_eq_dec (a b : field) : {a = b} + {a <> b}.
 Proof. decide equality; (apply Nat.eq_dec || decide equality). Defined.
+Definition transform_eq_dec (a b : transform) : {a = b} + {a <> b}.
+Proof.
+  decide equality;
+    (apply Nat.eq_dec || apply Bool.bool_dec || apply (list_eq_dec Nat.eq_dec)).
+Defined.
+
 Definition matchcond_eq_dec (a b : matchcond) : {a = b} + {a <> b}.
 Proof.
   decide equality;
     try (apply list_eq_dec; apply Nat.eq_dec);
     try (apply list_eq_dec; apply list_eq_dec; apply Nat.eq_dec);
+    try (apply list_eq_dec; apply transform_eq_dec);
     try apply field_eq_dec;
     try apply Bool.bool_dec;
     try apply string_dec.
